txn-data-consistency/Reductions.thy
@@ -239,7 +239,7 @@ definition inverted_pairs :: "('e \<Rightarrow> 'a :: linorder option) \<Rightar
   "inverted_pairs f tr = 
     {(i, j) | i j c1 c2. i < j \<and> j < length tr \<and> f(tr ! i) = Some c2 \<and> f(tr ! j) = Some c1 \<and> c2 > c1}"
 
-abbreviation adj_inv_pair where
+definition adj_inv_pair where
   "adj_inv_pair f tr i j \<equiv> (i, j) \<in> inverted_pairs f tr \<and>
     (\<forall>l. i < l \<and> l < j \<longrightarrow>
       (i, l) \<notin> inverted_pairs f tr \<and>
@@ -268,7 +268,7 @@ lemma inverted_pairs_i_lt_j:
 
 lemma adj_inv_eq_all_none:
   "adj_inv_pair f tr i j \<longleftrightarrow> (i, j) \<in> inverted_pairs f tr \<and> (\<forall>l. i < l \<and> l < j \<longrightarrow> f (tr ! l) = None)"
-  apply (auto simp add: inverted_pairs_def)
+  apply (auto simp add: adj_inv_pair_def inverted_pairs_def)
   by (meson dual_order.strict_trans1 linorder_le_less_linear option.exhaust)
 
 lemma adj_inv_exists_n:
@@ -276,7 +276,8 @@ lemma adj_inv_exists_n:
    \<exists>i j. adj_inv_pair f tr i j"
   apply (induction n rule: nat_less_induct, auto)
   subgoal for i j
-    apply (cases "adj_inv_pair f tr i j", auto)
+    apply (cases "adj_inv_pair f tr i j", auto simp add: adj_inv_pair_def)
+    apply (metis adj_inv_pair_def)
     using diff_less_mono order_less_imp_le apply blast
     using diff_less_mono2 order.strict_trans by blast.
 
@@ -293,7 +294,7 @@ lemma lmp_is_inverted:
   assumes "\<exists>i j. adj_inv_pair f tr i j"
   shows "left_most_adj_pair f tr = (a, b) \<Longrightarrow> (a, b) \<in> inverted_pairs f tr"
   using assms
-  apply (auto simp add: left_most_adj_pair_def)
+  apply (auto simp add: left_most_adj_pair_def adj_inv_pair_def)
   by (smt (verit) arg_min_natI case_prod_conv)
 
 lemma inverted_pairs_append: "inverted_pairs f (tr @ [e]) =  inverted_pairs f tr \<union>
